spc/Hoareproof0.v
@@ -117,16 +117,16 @@ Section CANCEL.
 
   Context `{Σ: GRA.t}.
 
-  Variable md: SMod.t.
+  Variable mds: list SMod.t.
 
-  Let sk: Sk.t := Sk.sort (Sk.add Sk.unit (SMod.sk md)).
+  Let sk: Sk.t := Sk.sort (fold_right Sk.add Sk.unit (List.map SMod.sk mds)).
   (* Let skenv: SkEnv.t := Sk.load_skenv sk. *)
 
-  Let _ms: Sk.t -> SModSem.t := fun sk => (SMod.get_modsem md sk).
-  Let _sbtb: Sk.t -> list (gname * fspecbody) := fun sk => ((SModSem.fnsems) (_ms sk)).
+  Let _mss: Sk.t -> list SModSem.t := fun sk => (List.map ((flip SMod.get_modsem) sk) mds).
+  Let _sbtb: Sk.t -> list (gname * fspecbody) := fun sk => (List.flat_map (SModSem.fnsems) (_mss sk)).
   Let _stb: Sk.t -> list (gname * fspec) := fun sk => List.map (fun '(fn, fs) => (fn, fs.(fsb_fspec))) (_sbtb sk).
 
-  Let ms: SModSem.t := _ms sk.
+  Let mss: list SModSem.t := _mss sk.
   Let sbtb: list (gname * fspecbody) := _sbtb sk.
 
   Variable stb: Sk.t -> gname -> option fspec.
@@ -140,40 +140,57 @@ Section CANCEL.
   (* Let sbtb: list (gname * fspecbody) := (List.flat_map (SModSem.fnsems) mss). *)
   (* Let stb: list (gname * fspec) := List.map (fun '(fn, fs) => (fn, fs.(fsb_fspec))) sbtb. *)
 
-  Let md_mid: Mod.t := (SMod.to_mid (stb sk)) md.
-  Let md_tgt: Mod.t := (SMod.to_tgt stb) md.
+  Let mds_mid: list Mod.t := List.map (SMod.to_mid (stb sk)) mds.
+  Let mds_tgt: list Mod.t := List.map (SMod.to_tgt stb) mds.
+
+
+  Let md_mid: Mod.t := Mod.add_list mds_mid.
+  Let md_tgt: Mod.t := Mod.add_list mds_tgt.
 
   Let ms_mid: ModSem.t := Mod.enclose md_mid.
   Let ms_tgt: ModSem.t := Mod.enclose md_tgt.
 
 
+  Import ModSem.
+
   Lemma sk_eq:
     Mod.sk md_tgt = Mod.sk md_mid.
-  Proof. ss. Qed.
+  Proof. 
+    unfold md_tgt, md_mid, mds_tgt, mds_mid.
+    rewrite ! ModFacts.add_list_sk. f_equal.
+    generalize mds. clear. i. induction mds0; ss. 
+    rewrite IHmds0. ss.
+  Qed.
 
   (* Lemma fst_initial_mrs_eq:
-    fst (ModSem.init_st ms_tgt) = fst ModSem.init_st ms_mid.
+    init_st ms_tgt = init_st ms_mid.
   Proof.
     pose proof sk_eq.
-    unfold ms_tgt, ms_mid, mds_tgt, mds_mid, ModL.enclose.
-    unfold mds_mid, mds_tgt in H. rewrite H.
-    generalize (ModL.sk (Mod.add_list (List.map (SMod.to_mid (stb sk)) mds))). i.
-    rewrite ! Mod.add_list_initial_mrs.
-    generalize mds. clear. i. induction mds0; auto.
-    ss. rewrite IHmds0. auto.
+    unfold ms_mid, ms_tgt, md_mid, md_tgt, mds_mid, mds_tgt, Mod.enclose.
+    unfold md_mid, md_tgt, mds_mid, mds_tgt in H. rewrite H.
+    generalize (Mod.sk (Mod.add_list (List.map (SMod.to_mid (stb sk)) mds))). i.
+    rewrite ! ModFacts.add_list_initial_mrs.
+    generalize mds. clear. i. 
+    induction mds0; et.
+    destruct mds0.
+    - s.
+    rewrite IHmds0. ss.
   Qed. *)
 
   Lemma fns_eq:
-    (List.map fst (ModSem.fnsems (Mod.enclose md_tgt)))
+    (List.map fst (fnsems (Mod.enclose (md_tgt))))
     =
-    (List.map fst (ModSem.fnsems (Mod.enclose md_mid))).
+    (List.map fst (fnsems (Mod.enclose (md_mid)))).
   Proof.
     pose proof sk_eq. unfold Mod.enclose.
-    unfold md_mid, md_tgt, Mod.enclose.
-    unfold md_mid, md_tgt in H. rewrite H.
-    ss. rewrite ! List.map_map. f_equal.
+    unfold md_tgt, md_mid, mds_tgt, mds_mid, Mod.enclose.
+    unfold md_tgt, md_mid, mds_tgt, mds_mid in H. rewrite H.
+    generalize (Mod.sk (Mod.add_list (List.map (SMod.to_mid (stb sk)) mds))). i.
+    rewrite ! ModFacts.add_list_fns. rewrite ! List.map_map. f_equal. 
+    f_equal. extensionality sm. ss. rewrite ! List.map_map. f_equal.
     extensionality fnsb. destruct fnsb as [fn sb]. ss.
   Qed.
+
 
   Lemma stb_find_iff_aux fn
     :
@@ -181,24 +198,63 @@ Section CANCEL.
        (<<FINDMID: alist_find fn (ModSem.fnsems ms_mid) = None>>) /\
        (<<FINDTGT: alist_find fn (ModSem.fnsems ms_tgt) = None>>)) \/
 
-      (exists (f: fspecbody),
+      (exists (f: fspecbody) (run_: RUN),
           (<<STB: alist_find fn (_stb sk) = Some (f: fspec)>>) /\
           (<<SBTB: alist_find fn sbtb = Some f>>) /\
           (<<FINDMID: alist_find fn (ModSem.fnsems ms_mid) =
-                      Some (fun_to_mid (stb sk) (fsb_body f))>>) /\
+                      Some ((translate (emb_ run_)  (T:=Any.t)) ∘ fun_to_mid (stb sk) (fsb_body f))>>) /\
           (<<FINDTGT: alist_find fn (ModSem.fnsems ms_tgt) =
-                      Some (fun_to_tgt (stb sk) f)>>)).
+                      Some ((translate (emb_ run_)  (T:=Any.t)) ∘ fun_to_tgt (stb sk) f)>>)).
           (* (<<MIN: List.In (SModSem.mn (SMod.get_modsem md sk)) (List.map fst ms_tgt.(ModSemL.initial_mrs))>>)). *)
   Proof.
-    unfold ms_mid, ms_tgt, md_tgt, md_mid, SMod.to_mid, md_tgt, SMod.to_tgt.
-    rewrite SMod.transl_fnsems. rewrite SMod.transl_fnsems. fold sk. 
+    unfold ms_mid, ms_tgt, md_tgt, md_mid, mds_tgt, mds_mid, SMod.to_mid, md_tgt, SMod.to_tgt.
+    rewrite ! SMod.transl_fnsems. fold sk. 
     (* rewrite SMod.transl_init_st.  *)
-    unfold _stb at 1 2. unfold sbtb, _sbtb, _ms. 
-    unfold SMod.load_fnsems. rewrite ! SMod.red_do_ret2.
-    rewrite ! alist_find_map. uo.
-    destruct (alist_find fn (SModSem.fnsems (SMod.get_modsem md sk))) eqn:FIND.
-    { right. esplits; et. }
-    { left. esplits; et. }
+    unfold _stb at 1 2. unfold sbtb, _sbtb, _mss. rewrite alist_find_map.
+    generalize mds. induction mds0; ss; auto. unfold SMod.get_fnsems.
+    rewrite ! alist_find_app_o. erewrite ! SMod.red_do_ret2. uo.
+    destruct (alist_find fn (SModSem.fnsems (SMod.get_modsem a sk))) eqn: AFIND.
+    { 
+      right. destruct mds0.
+      { 
+        rewrite ! alist_find_map. uo.  rewrite AFIND.
+        exists f. exists run_id. 
+        (* esplits; et.
+        { unfold run_id. f_equal. apply func_ext. i. erewrite (bisimulation_is_eq _ _ (translate_id _ _ _)). } *)
+        esplits; et; (f_equal; apply func_ext; i; rewrite <- emb_run_id; rewrite emb_id_eq; refl).
+      }
+      { 
+        unfold trans_l, trans_r. rewrite ! alist_find_app_o.
+        rewrite ! alist_find_map. uo. rewrite AFIND.
+        esplits; et. 
+      }
+    }
+    { 
+      destruct mds0. 
+      { s. rewrite ! alist_find_map. uo. rewrite AFIND. left. esplits; et. }
+      { 
+        s. unfold trans_l, trans_r. rewrite ! alist_find_app_o.
+        rewrite ! alist_find_map. uo. rewrite AFIND. 
+        s in IHmds0. unfold SMod.get_fnsems, trans_l, trans_r in IHmds0.
+        rewrite ! alist_find_app_o in IHmds0. erewrite ! SMod.red_do_ret2 in IHmds0.
+        des.
+        { 
+          left. esplits; et; unfold SMod.get_fnsems; rewrite SMod.red_do_ret2.
+          - rewrite FINDMID. refl.
+          - rewrite FINDTGT. refl.        
+        }
+        {
+          right. exists f. esplits; et; unfold SMod.get_fnsems; rewrite SMod.red_do_ret2. 
+          - rewrite FINDMID.
+            f_equal. apply func_ext. i. erewrite <- (bisimulation_is_eq _ _ (translate_cmpE _ _ _ _ _ _ _)).
+            replace emb_r with (emb_ run_r); ss.
+            repeat f_equal. unfold emb_. unfold ">>>", Cat_IFun. extensionalities. des_ifs.
+          - rewrite FINDTGT.
+            f_equal. apply func_ext. i. erewrite <- (bisimulation_is_eq _ _ (translate_cmpE _ _ _ _ _ _ _)).
+            repeat f_equal. unfold emb_, emb_r, ">>>", Cat_IFun. extensionalities. des_ifs.
+        }
+      }
+    }
   Qed.
 
   Lemma stb_find_iff fn
@@ -207,13 +263,13 @@ Section CANCEL.
        (<<FINDMID: alist_find fn (ModSem.fnsems ms_mid) = None>>) /\
        (<<FINDTGT: alist_find fn (ModSem.fnsems ms_tgt) = None>>)) \/
 
-      (exists (f: fspecbody),
+      (exists (f: fspecbody) (run_: RUN),
           (<<STB: stb sk fn = Some (f: fspec)>>) /\
           (<<SBTB: alist_find fn sbtb = Some f>>) /\
           (<<FINDMID: alist_find fn (ModSem.fnsems ms_mid) =
-                      Some (fun_to_mid (stb sk) (fsb_body f))>>) /\
+                      Some ((translate (emb_ run_)  (T:=Any.t)) ∘ fun_to_mid (stb sk) (fsb_body f))>>) /\
           (<<FINDTGT: alist_find fn (ModSem.fnsems ms_tgt) =
-                      Some (fun_to_tgt (stb sk) f)>>)). 
+                      Some ((translate (emb_ run_)  (T:=Any.t)) ∘ fun_to_tgt (stb sk) f)>>)). 
   Proof.
     hexploit (stb_find_iff_aux fn). i. des.
     { left. esplits; et. }
@@ -391,12 +447,78 @@ Section CANCEL.
   Qed. *)
 
 
+  (************** Temporary tactics. ***************)
+  (* Ltac steps := repeat (mred; try _step ltac:(guclo simg_safe_spec); des_ifs_safe). *)
+
+  Ltac a1 := try rewrite ! Any.pair_split.
+  Ltac a2 := try rewrite ! Any.upcast_downcast.
+
+  Ltac t1 := try rewrite ! translate_emb_bind.
+  Ltac t2 := try rewrite ! translate_emb_ret.
+  Ltac t3 := try rewrite ! translate_emb_tau.
+  Ltac t4 := try rewrite translate_emb_callE.
+  Ltac t5 := try rewrite translate_emb_eventE.
+  Ltac t6 := try rewrite translate_emb_sE.
+  Ltac t7 := try rewrite translate_emb_triggerUB.
+  Ltac t8 := try rewrite translate_emb_triggerNB.
+
+  Ltac tset := t1; t2; t3; t4; t5; t6; t7; t8.
+
+  Ltac m1 := try rewrite ! interp_mid_bind.
+  Ltac m2 := try rewrite ! interp_mid_ret.
+  Ltac m3 := try rewrite ! interp_mid_tau.
+  Ltac m4 := try rewrite interp_mid_hcall.
+  Ltac m5 := try rewrite interp_mid_triggere.
+  Ltac m6 := try rewrite interp_mid_triggerp.
+
+  Ltac mset := m1; m2; m3; m4; m5; m6.
+
+  Ltac n1 := try rewrite ! interp_tgt_bind.
+  Ltac n2 := try rewrite ! interp_tgt_ret.
+  Ltac n3 := try rewrite ! interp_tgt_tau.
+  Ltac n4 := try rewrite interp_tgt_hcall.
+  Ltac n5 := try rewrite interp_tgt_triggere.
+  Ltac n6 := try rewrite interp_tgt_triggerp.
+
+  Ltac nset := n1; n2; n3; n4; n5; n6.
+
+
+  Ltac h1 := try rewrite ! interp_hEs_tgt_bind.
+  Ltac h2 := try rewrite ! interp_hEs_tgt_ret.
+  Ltac h3 := try rewrite ! interp_hEs_tgt_tau.
+  Ltac h4 := try rewrite ! interp_hEs_tgt_hapc.
+  Ltac h5 := try rewrite interp_hEs_tgt_triggere.
+  Ltac h6 := try rewrite interp_hEs_tgt_triggerp.
+
+  Ltac hset := h1; h2; h3; h4; h5; h6.
+
+
+  Ltac tstep := repeat (unfold guarantee; a1; a2; tset; steps).
+  Ltac mstep := repeat (unfold guarantee; a1; a2; tset; nset; steps).
+  Ltac nstep := repeat (unfold guarantee; a1; a2; tset; mset; nset; steps).
+  Ltac hstep := repeat (unfold guarantee; a1; a2; tset; mset; nset; hset; steps).
+
+
+  Definition run_tgt: RUN := 
+  fun _ run x =>
+    match Any.split x with
+    | Some (st, mr) => ((Any.pair (run st).1 mr), (run st).2)
+    | None => run tt↑
+    end.
+
+  Hypothesis RUN_TGT: forall X x run (run_: RUN), run_ X (run_tgt run) x = run_tgt (run_ X run) x. 
+
+  Hypothesis RUN_STATE: forall X x run (run_: RUN), snd (run_ X run x) = snd (run x).
+
+  Hypothesis RUN_PUT: forall x (run_: RUN), run_ unit (rPut x) = rPut x.
+
   Let adequacy_type_aux:
     forall RT
            mr0 frs 
            ctx0
            st_src0 st_tgt0 (i0: itree (hCallE +' sE +' eventE) RT)
            cur
+           (run_: RUN)
            (ZIP: st_tgt0 = zip_state st_src0 mr0)
            (CTX: ctx0 = frs)
            (* (CTX: ctx0 = frs ⋅ mr0) *)
@@ -404,11 +526,12 @@ Section CANCEL.
       simg (fun '(st_src1, v_src) '(st_tgt1, v_tgt) =>
               exists mrs1,
                 (<<ZIP: st_tgt1 = zip_state st_src1 mrs1>>) /\
+                
                 (<<RET: (v_tgt: Σ * RT) = (frs, v_src)>>))
                 (* (<<RET: (v_tgt: Σ * RT) = (frs ⋅ mrs1, v_src)>>)) *)
            false false
-           (interp_Es (ModSem.prog ms_mid) (interp_hCallE_mid (stb sk) cur i0) st_src0)
-           (interp_Es (ModSem.prog ms_tgt) (interp_hCallE_tgt (stb sk) cur i0 ctx0) st_tgt0)
+           (interp_Es (ModSem.prog ms_mid) (translate (emb_ run_) (interp_hCallE_mid (stb sk) cur i0)) st_src0)
+           (interp_Es (ModSem.prog ms_tgt) (translate (emb_ run_) (interp_hCallE_tgt (stb sk) cur i0 ctx0)) st_tgt0)
   .
   Proof.
   (* Admitted. *)
@@ -417,23 +540,31 @@ Section CANCEL.
     { i. eapply cpn7_wcompat; eauto with paco. }
     gcofix CIH. i; subst.
     ides i0; try rewrite ! unfold_interp; cbn; mred.
-    { steps. }
-    { steps. deflag. gbase. eapply CIH; [..|M]; Mskip et. ss. }
+    { nstep. }
+    { nstep. deflag. gbase. eapply CIH; [..|M]; Mskip et. ss. }
     rewrite <- bind_trigger. destruct e; cycle 1.
     {
       destruct s; ss.
       {
         destruct s; ss.
-        resub. steps. unfold pupdate. steps. deflag.
-        unfold zip_state in Heq0. rewrite Any.pair_split in Heq0. 
+        resub. nstep. unfold pupdate. nstep. deflag.
+        
+        unfold zip_state in Heq0.
+        replace (λ st : Any.t, match Any.split st with
+        | Some p => let (x, mr) := p in (Any.pair (run x).1 mr, (run x).2)
+        | None => run (Any.upcast ())
+        end) with (run_tgt run) in Heq0; ss.
+        rewrite RUN_TGT in Heq0. unfold run_tgt in Heq0.
+        
+        rewrite Any.pair_split in Heq0. 
         rewrite Heq in Heq0. clarify.
-        gbase. eapply CIH; ss.
+        gbase. eapply CIH; ss. 
       }
       { dependent destruction e.
-        - resub. ired_both. force_r. steps. esplits; eauto. steps. deflag.
+        - resub. repeat (try nset; try tset). rewrite ! interp_Es_bind. rewrite interp_Es_eventE. grind. force_r. nstep. esplits. nstep. deflag.
           gbase. eapply CIH; [..|M]; Mskip et. ss.
-        - resub. steps. esplits; eauto. steps. deflag. gbase. eapply CIH; [..|M]; Mskip et. ss.
-        - resub. steps. deflag. gbase. eapply CIH; [..|M]; Mskip et. ss.
+        - resub. nstep. esplits; eauto. nstep. deflag. gbase. eapply CIH; [..|M]; Mskip et. ss.
+        - resub. nstep. deflag. gbase. eapply CIH; [..|M]; Mskip et. ss.
       }
     }
     dependent destruction h. resub.
@@ -442,46 +573,70 @@ Section CANCEL.
     ss.
     seal_left.
 
-    steps. hexploit (stb_find_iff fn). i. des.
-    { rewrite NONE. steps. }
-    { rewrite FIND. unfold HoareCall, ASSUME, ASSERT, mput, mget. steps.
-      unfold zip_state. steps.
+    mstep. hexploit (stb_find_iff fn). i. des.
+    { rewrite NONE. nstep. }
+    { rewrite FIND. unfold HoareCall, ASSUME, ASSERT, mput, mget. 
+      unfold unwrapN.
+      mstep.
+      unfold zip_state, sGet, sPut.
+      mstep.
+      hexploit (RUN_STATE (Any.pair st_src0 (Any.upcast mr0)) rGet run_). i.
+      rewrite Heq in H. s in H.
+      rewrite H.
+      rewrite Any.pair_split.
+      mstep.
+
       des; clarify. destruct tbr; ss.
       { exfalso. hexploit TRIVIAL; et. intro T. rewrite T in *. hexploit x4; ss. }
-      seal_right. unseal_left. steps. rewrite FIND. steps. esplits; et.
-      steps. esplits; et.
-      { destruct cur; ss. hexploit x5; ss. intro T. rewrite T in *; ss. }
-      steps. rewrite FINDMID. steps.
+      seal_right. unseal_left. nstep. rewrite FIND. nstep. esplits; et.
+      nstep. esplits; et.
+      (* { destruct cur; ss. hexploit x5; ss. intro T. rewrite T in *; ss. } *)
+      nstep. rewrite FINDMID. nstep.
     }
     unfold HoareCall, ASSUME, ASSERT, mput, mget.
 
     (*** exploiting both_tau ***)
-    rewrite STB. ss. mred. force_r.
+    rewrite STB. ss.
+    tset. rewrite interp_Es_ret. steps.
+    tset. rewrite interp_Es_bind. rewrite interp_Es_eventE.
+    grind.
+    
+    force_r.
     destruct (classic (tbr = true /\ forall x, f.(measure) x = ord_top)).
-    { des. subst. steps.
-      unfold zip_state. rewrite Any.pair_split. steps.
+    { des. subst. nstep.
+      unfold zip_state. unfold unwrapN, sGet, sPut. nstep.
+      hexploit (RUN_STATE (Any.pair st_src0 (Any.upcast mr0)) rGet run_). i.
+      rewrite Heq0 in H. s in H. rewrite H. nstep. 
+
       hexploit H0; et. i. rewrite H in *. ss. des. hexploit x4; ss. }
     rename H into TRIVIAL.
-    unseal_left. ired_both. rewrite STB. steps. esplit.
-    { ii. subst. eapply TRIVIAL; ss. } steps.
-    unfold zip_state. rewrite Any.pair_split. steps.
-
+    unseal_left. ired_both. 
+    mset. tset. ired_l. tset. rewrite interp_Es_tau.
+    
+    rewrite STB. nstep. esplit.
+    (* { ii. subst. eapply TRIVIAL; ss. }  *)
+    nstep.
+    unfold zip_state, sGet, sPut. nstep.
+    hexploit (RUN_STATE (Any.pair st_src0 (Any.upcast mr0)) rGet run_). i.
+    rewrite Heq in H. s in H. rewrite H. rewrite Any.pair_split.
+    nstep.
+     
     match goal with
     | |- _ ?i_tgt => replace i_tgt with (Ret tt;;; i_tgt)
     end.
-    2: { mred. auto. }
+    2: { nstep. }
     deflag. guclo bindC_spec. econs.
     { instantiate (1:= fun '(st_src, o) (_: unit) => st_src = st_src0 /\ o = (f.(measure) x)).
       destruct tbr.
-      { steps. des. destruct (measure f x); ss.
-        { exists n. steps. }
+      { nstep. des. destruct (measure f x); ss.
+        { exists n. nstep. }
         { exfalso. hexploit x4; ss. }
       }
-      { steps. des. splits; auto. symmetry. auto. }
+      { nstep. des. splits; auto. symmetry. auto. }
     }
     i. destruct vret_src, vret_tgt. des; subst.
 
-    steps. esplits; eauto. steps. unfold unwrapU.
+    nstep. esplits; eauto. nstep. unfold unwrapU.
     rewrite FINDMID. rewrite FINDTGT. rewrite ! bind_ret_l.
 
     guclo bindC_spec. econs.
@@ -496,34 +651,64 @@ Section CANCEL.
       fold Any_tgt in x3.
       unfold fun_to_mid, fun_to_tgt, compose. des_ifs. unfold HoareFun, ASSUME, ASSERT, mget, mput.
       rename x3 into PRECOND. rename c0 into rarg.
-      steps. exists x.
-      steps. eexists (rarg, c1 ⋅ (frs)). steps.
+      nstep. exists x.
+      nstep. eexists (rarg, c1 ⋅ (frs)). nstep.
       (* erewrite ! zip_state_mput; et. steps. *)
       assert (RWF0: URA.wf (rarg ⋅ ε ⋅ (c1 ⋅ (frs)) ⋅ c)).
       { r_wf x0. }
-      unshelve esplits; eauto. steps.
+      unshelve esplits; eauto.
+      unfold sGet, sPut. nstep.
+      hexploit (RUN_STATE t1 rGet run_0). i.
+      rewrite Heq1 in H. s in H. rewrite H.
+
+
+      rewrite RUN_PUT in Heq0.
+      assert (t1 = Any.pair st_src0 c↑). { unfold rPut in Heq0. clarify. }
+      nstep. unfold assume. nstep. eexists.
+      nstep.
+
       exists varg_src.
-      steps. esplits; eauto. steps. unshelve esplits; eauto. steps.
+      nstep. esplits; eauto. nstep. unshelve esplits; eauto. nstep.
       deflag. guclo bindC_spec. econs.
-      { gbase. eapply CIH; ss.
+      { gbase. eapply CIH; ss. admit. (* st_tgt form *)
       }
       { ii. ss. des_ifs_safe. des; ss. clarify.
-        steps.
-        unfold zip_state.
-        rewrite Any.pair_split. steps.
+        nstep.
+        unfold zip_state. nstep.
+        assert (t5 = (zip_state t1 mrs1)).
+        { 
+          replace (zip_state t1 mrs1) with (run_0 Any.t rGet (zip_state t1 mrs1)).2.
+          2: { erewrite RUN_STATE. et. }
+          rewrite Heq2. ss.
+        }
+        
+        nstep. unfold zip_state. nstep.
         esplits; ss; et.
+        { rewrite RUN_PUT in Heq3. unfold rPut in Heq3. inv Heq3. et. }
         { eapply (@URA.wf_mon _ _ c3). r_wf x3. }
       }
     }
     { ii. ss. des_ifs_safe. des. subst.
-      steps. eexists (rret, frs). steps.
-      unfold zip_state.
+      nstep. eexists (rret, frs). nstep.
+      replace t6 with (Any.pair t2 mr1↑). 
+      2: {  
+          replace t6 with (run_ Any.t rGet (zip_state t2 mr1)).2. 
+          { rewrite RUN_STATE. ss. }
+          { rewrite Heq1. ss. }
+      }
+
+      
       (* rewrite zip_state_get; et. *)
-      rewrite Any.pair_split. steps. rewrite Any.upcast_downcast. steps.
-      unshelve esplits; et.
+      rewrite Any.pair_split. nstep.
+      unfold assume. nstep. 
+      (* rewrite Any.upcast_downcast. steps. *)
+      unshelve esplits; et. 
+
       { r_wf RWF. }
-      steps. exists t0. steps. unshelve esplits; et.
-      steps. deflag. gbase. eapply CIH; et.
+      nstep. exists t3. nstep. unshelve esplits; et.
+       (* { admit. } *)
+      nstep. deflag. gbase. eapply CIH; et.
+
     }
   Unshelve.
     all: try (by exact 0).
@@ -541,7 +726,7 @@ Section CANCEL.
              forall (main_fsp: fspec) (MAIN: stb sk "main" = Some main_fsp),
              exists (x: main_fsp.(meta)) entry_r,
                (<<PRE: main_fsp.(precond) x (@initial_arg CONFS) (@initial_arg CONFT) entry_r ∧ main_fsp.(measure) x = ord_top>>) /\
-               (<<WFR: URA.wf (entry_r ⋅ (SModSem.initial_mr ms))>>) /\
+               (<<WFR: URA.wf (entry_r ⋅ fold_left (⋅) (List.map SModSem.initial_mr mss) ε)>>) /\
                (<<RET: forall ret_src ret_tgt r
                               (WFR: URA.wf r)
                               (POST: main_fsp.(postcond) x ret_src ret_tgt r),
@@ -568,7 +753,7 @@ Section CANCEL.
     { inv WF. rewrite fst_initial_mrs_eq. unfold ms_mid. auto. } *)
     esplits; et.
     { inv WF. econs; auto. rewrite fns_eq. auto. }
-    (* { rewrite sk_eq. auto. } *)
+    { rewrite sk_eq. auto. }
     
 
     (* hexploit initial_mrs_exist; auto. i. des. *)
@@ -576,13 +761,29 @@ Section CANCEL.
      (* rewrite <- INITIALZIP. *)
 
     Local Transparent ModSem.prog. ss.
-    unfold Any_src, Any_mid, Any_tgt in *. rewrite FINDTGT. rewrite FINDMID. unfold fun_to_mid, fun_to_tgt, HoareFun. steps.
-    eexists. steps. unfold ASSUME, ASSERT, mput, mget. steps.
+    unfold Any_src, Any_mid, Any_tgt in *. rewrite FINDTGT. rewrite FINDMID.
+    unfold fun_to_mid, fun_to_tgt, HoareFun. nstep.
+     
+    eexists. nstep. unfold ASSUME, ASSERT, mput, mget. nstep.
     eexists (entry_r, ε).
     (* eexists (entry_r, (SMod.get_modsem md sk).(SModSem.initial_mr)). *)
-    steps.  
-    (* rewrite zip_state_get; et. steps. *)
-    assert (RWF: URA.wf (entry_r ⋅ ε ⋅ ε ⋅ (SMod.get_modsem md sk).(SModSem.initial_mr))).
+    unfold sGet, sPut.
+    nstep.  
+
+    hexploit (RUN_STATE (init_st ms_tgt) rGet run_). i.
+    rewrite Heq in H. s in H. rewrite H.
+    destruct (Any.split (init_st ms_tgt)).
+    2: { nstep. admit. }
+    
+    nstep.
+    destruct (Any.downcast t2).
+    2: { nstep. admit. }
+    unfold assume. nstep.
+
+    assert (RWF: URA.wf (entry_r ⋅ ε ⋅ ε ⋅ fold_left URA.add (map SModSem.initial_mr mss) ε)).
+    (* assert (RWF: URA.wf (entry_r ⋅ ε ⋅ ε ⋅ (SMod.get_modsem md sk).(SModSem.initial_mr))). *)
+
+
     (* assert (RWF: URA.wf (entry_r ⋅ ε ⋅ (SMod.get_modsem md sk).(SModSem.initial_mr) ⋅ (SMod.get_modsem md (Sk.sort (SMod.sk md))).(SModSem.initial_mr))). *)
     { r_wf WFR. 
       (* unfold ms, _ms.
@@ -591,19 +792,23 @@ Section CANCEL.
       (* admit. *)
         }
     unshelve esplits; et.
-    steps.
-    eexists. steps. unshelve esplits; et. steps.
+    { admit. }
+    nstep.
+    eexists. nstep. unshelve esplits; et. nstep.
     guclo bindC_spec. econs.
     { deflag. gfinal. right. fold simg.
       (* admit. *)
-      eapply adequacy_type_aux; ss.
+      eapply adequacy_type_aux; ss. admit.
     }
     i. ss.
     destruct vret_src as [mps_src v_src].
     destruct vret_tgt as [mps_tgt [? v_tgt]]. des. clarify.
-    steps.
-    unfold zip_state.
-    rewrite Any.pair_split. steps.
+    nstep.
+
+    hexploit (RUN_STATE (zip_state mps_src mrs1) rGet run_). i.
+    rewrite Heq1 in H. s in H. rewrite H.
+
+    unfold zip_state. nstep.
     { eapply RET; [|et]. eapply URA.wf_mon.
       instantiate (1:=(c1 ⋅ ε ⋅ c)).
       r_wf x0. }
